\setchapterpreamble[u]{\margintoc}
\chapter[Rotation of the quadrupole tensor around the z-axis]{Rotation of the quadrupole tensor around the $z$-axis}
\label{app:rotations_quadrupole}

We start from the Cartesian, symmetric traceless tensor

\begin{equation}
Q=\begin{pmatrix}
Q_{xx} & Q_{xy} & Q_{xz}\\
Q_{xy} & Q_{yy} & Q_{yz}\\
Q_{xz} & Q_{yz} & Q_{zz}
\end{pmatrix},\qquad \mathrm{Tr}\,Q=0,
\end{equation}

and rotate the axes by an angle $\phi$ about $z$ with

\begin{equation}
R_z(\phi)=
\begin{pmatrix}
\cos\phi & \sin\phi & 0\\
-\sin\phi & \cos\phi & 0\\
0 & 0 & 1
\end{pmatrix}.
\end{equation}
Under this passive rotation,
\begin{equation}
Q' \;=\; R_z(\phi)\,Q\,R_z^\top(\phi).
\end{equation}

Carrying out the multiplication gives

\begin{equation}
\begin{aligned}
Q'_{xx} &= \cos^2\!\phi\,Q_{xx}+\sin^2\!\phi\,Q_{yy}+2\sin\phi\cos\phi\,Q_{xy},\\
Q'_{yy} &= \sin^2\!\phi\,Q_{xx}+\cos^2\!\phi\,Q_{yy}-2\sin\phi\cos\phi\,Q_{xy},\\
Q'_{xy} &= (\cos^2\!\phi-\sin^2\!\phi)\,Q_{xy}+\sin\phi\cos\phi\,(Q_{yy}-Q_{xx}),\\
Q'_{xz} &= \cos\phi\,Q_{xz}+\sin\phi\,Q_{yz},\\
Q'_{yz} &= -\sin\phi\,Q_{xz}+\cos\phi\,Q_{yz},\\
Q'_{zz} &= Q_{zz}.
\end{aligned}
\label{eq:Qprime-cart}
\end{equation}

We define the spherical components (rank-2 irreducible combinations) as

\begin{equation}
\begin{aligned}
Q_0 &= Q_{zz},\\
Q_{\pm1} &= Q_{xz}\pm iQ_{yz},\\
Q_{\pm2} &= \tfrac12\,(Q_{xx}-Q_{yy}) \pm i\,Q_{xy}.
\end{aligned}
\label{eq:Q-spherical-def}
\end{equation}

Using \ref{eq:Qprime-cart} in the definition of $Q'_{\pm1}$,

\begin{equation}
\begin{aligned}
Q'_{+1}
&= Q'_{xz}+i\,Q'_{yz}\\
&= \big(\cos\phi\,Q_{xz}+\sin\phi\,Q_{yz}\big)\;+\;i\big(-\sin\phi\,Q_{xz}+\cos\phi\,Q_{yz}\big)\\
&= (\cos\phi - i\sin\phi)\,Q_{xz}\;+\;(\sin\phi + i\cos\phi)\,Q_{yz} =\; e^{-i\phi}\,Q_{+1}.
\end{aligned}
\end{equation}

Similarly,

\begin{equation}
\begin{aligned}
Q'_{-1}
&= Q'_{xz}-i\,Q'_{yz}\\
&= \big(\cos\phi\,Q_{xz}+\sin\phi\,Q_{yz}\big)\;-\;i\big(-\sin\phi\,Q_{xz}+\cos\phi\,Q_{yz}\big)\\
&= (\cos\phi + i\sin\phi)\,Q_{xz}\;+\;(\sin\phi - i\cos\phi)\,Q_{yz}\\
&= e^{+i\phi}\,\big(Q_{xz}-iQ_{yz}\big) \;=\; e^{+i\phi}\,Q_{-1}.
\end{aligned}
\end{equation}

Let $\Delta\equiv Q_{xx}-Q_{yy}$. From \eqref{eq:Qprime-cart},

\begin{equation}
\begin{aligned}
Q'_{+2}
&= \tfrac12\,(Q'_{xx}-Q'_{yy}) + i\,Q'_{xy}\\
&= \tfrac12\Big[\big(\cos^2\!\phi-\sin^2\!\phi\big)\Delta + 4\sin\phi\cos\phi\,Q_{xy}\Big]\\
&+ i\Big[\big(\cos^2\!\phi-\sin^2\!\phi\big)Q_{xy} - \sin\phi\cos\phi\,\Delta\Big].
\end{aligned}
\end{equation}

Use the double-angle identities $\cos 2\phi=\cos^2\!\phi-\sin^2\!\phi$ and $\sin 2\phi=2\sin\phi\cos\phi$ to rewrite
\begin{equation}
\begin{aligned}
Q'_{+2}
&= \tfrac12\Big[\cos 2\phi\,\Delta + 2\sin 2\phi\,Q_{xy}\Big]
+ i\Big[\cos 2\phi\,Q_{xy} - \tfrac12\sin 2\phi\,\Delta\Big]\\[4pt]
&= \left(\tfrac12\Delta + iQ_{xy}\right)\big(\cos 2\phi - i\sin 2\phi\big)\\[4pt]
&= \left(\tfrac12\Delta + iQ_{xy}\right) e^{-i2\phi}
\;=\; e^{-i2\phi}\,Q_{+2}.
\end{aligned}
\end{equation}

By complex conjugation or repeating the steps with $-i$,

\begin{equation}
Q'_{-2} \;=\; e^{+i2\phi}\,Q_{-2}.
\end{equation}

Since $Q'_{zz}=Q_{zz}$,
\begin{equation}
Q'_0 \;=\; Q_0.
\end{equation}

Collecting the results,

\begin{equation}
Q'_m \;=\; e^{-im\phi}\,Q_m,\qquad m=0,\pm1,\pm2.
\end{equation}

